working on equivalence.

src/ExprFacts.v
@@ -63,27 +63,52 @@ Section semantic.
     { change (t :: venv ++ ve) with ((t :: venv) ++ ve).
       erewrite IHe by eauto. reflexivity. }
   Qed.
- 
-  Theorem exprD_weaken_Some : forall ue ve e t venv x y, 
+
+  Fixpoint equiv_env (es1 es2 : env ts) : Prop :=
+    match es1 , es2 with
+      | nil , nil => True
+      | existT t1 v1 :: es1 , existT t2 v2 :: es2 =>
+        (exists pf : t2 = t1,
+          equiv ts t1 v1 match pf in _ = t return typD ts nil t with
+                           | eq_refl => v2 
+                         end)
+        /\ equiv_env es1 es2
+      | _ , _ => False
+    end.
+
+  Fixpoint equiv_hlist ls (h1 : hlist (typD ts (@nil Type)) ls) : hlist (typD ts (@nil Type)) ls -> Prop :=
+    match h1 in hlist _ ls return hlist (typD ts (@nil Type)) ls -> Prop with
+      | Hnil => fun _ => True
+      | Hcons t _ h1 hs1 => fun h2 => 
+        equiv ts t h1 (hlist_hd h2) /\ equiv_hlist _ hs1 (hlist_tl h2)
+    end.
+  Require Import RelationClasses.
+  Global Instance Reflexive_equiv_hlist ls : Reflexive (@equiv_hlist ls).
+  Proof.
+    red. induction x; simpl; auto.
+    split; auto. reflexivity.
+  Qed.
+  Global Instance Symmetric_equiv_hlist ls : Symmetric (@equiv_hlist ls).
+  Proof.
+    red. induction x; intros; rewrite (hlist_eta y) in *; simpl; auto.
+    simpl in H. destruct H. split; auto. symmetry. auto.
+  Qed.
+  Global Instance Transitive_equiv_hlist ls : Transitive (@equiv_hlist ls).
+  Proof.
+    red. induction x; intros; rewrite (hlist_eta y) in *; rewrite (hlist_eta z) in *; simpl; auto.
+    simpl in *. destruct H; destruct H0. split; try etransitivity; eauto.
+  Qed.
+
+  Require Import Morphisms.
+
+  
+
+  Theorem exprD'_weaken_Some : forall ue ve e t venv x y, 
     exprD' fs uenv venv e t = Some x ->
     exprD' fs (uenv ++ ue) (venv ++ ve) e t = Some y ->
     forall h he, equiv ts t (x h) (y (hlist_app h he)).
   Proof.
-  Admitted.
-    
-  Theorem exprD_weaken : forall venv e t ue ve x, 
-    exprD fs uenv venv e t = Some x ->
-    exists y, exprD fs (uenv ++ ue) (venv ++ ve) e t = Some y /\
-      equiv ts t x y.
-  Proof.
-    unfold exprD; intros. rewrite split_env_app.
-    destruct (split_env venv). destruct (split_env ve).
-    consider (exprD' fs uenv x0 e t); 
-    consider (exprD' fs (uenv ++ ue) (x0 ++ x1) e t); intros; try congruence.
-    { inversion H1; clear H1; subst.
-      revert h0. revert h.
-      generalize dependent x0; generalize dependent x1; generalize dependent t.
-      clear ve venv. induction e; simpl; intros;
+    induction e; simpl; intros;
       repeat match goal with
                | |- context [ match ?X with _ => _ end ] =>
                  match type of X with
@@ -104,26 +129,24 @@ Section semantic.
                           end
                  end
                | [ H : Some _ = Some _ |- _ ] => inversion H; clear H; subst
-             end; auto; try congruence.
-      { eexists; split; eauto. reflexivity. }
+             end; auto; try congruence; try reflexivity.
       { repeat match goal with
                  | [ H : context [ @refl_equal ?A ?B ] |- _ ] =>
                    generalize dependent (@refl_equal A B)
                end.
-        pattern (nth_error x0 v) at 2 3.
-        destruct (nth_error x0 v); try congruence.
-        intros. generalize dependent e.
-        generalize (nth_error_weaken x1 x0 _ e0); intro.
-        pattern (nth_error (x0 ++ x1) v) at 2 3.
-        rewrite H. intros.
-        consider (typ_eq_odec t2 t); intros; try congruence.
-        inversion H1; clear H1; inversion H2; clear H2; subst.
-        eexists; split; eauto.
+        pattern (nth_error venv v) at 2 3.
+        destruct (nth_error venv v); try congruence.
+        intros. generalize dependent e0.
+        generalize (nth_error_weaken ve venv _ e); intro.
+        pattern (nth_error (venv ++ ve) v) at 2 3.
+        rewrite H0. intros.
+        consider (typ_eq_odec t0 t); intros; try congruence.
+        inversion H1; inversion H2; clear H1 H2; subst.
         uip_all. clear.
         
         rewrite hlist_nth_hlist_app by eauto with typeclass_instances.
-        generalize (cast1 x0 x1 v).
-        generalize (cast2 x0 x1 v).
+        generalize (cast1 venv ve v).
+        generalize (cast2 venv ve v).
         uip_all.
         repeat match goal with
                  | |- context [ @eq_refl ?A ?B ] =>
@@ -145,35 +168,55 @@ Section semantic.
         rewrite (uip_refl _ e4).
         uip_all.
         clear.
-        generalize dependent (nth_error (x0 ++ x1) v).
+        generalize dependent (nth_error (venv ++ ve) v).
         intros; subst.
         rewrite (uip_refl _ e6).
         reflexivity. }
-      { eexists; split; eauto. clear.
-        generalize dependent (instantiate_typ (rev ts0) (ftype f0)). reflexivity. }
-      { admit. }
-      { eexists; split; eauto.
-        simpl; intro.
-        eapply IHe with (h := Hcons a h) (h0 := h0) in H0; eauto. 
-        destruct H0. destruct H0. inversion H0; clear H0; subst. auto. }        
-      { eexists; split; eauto.
-        unfold lookupAs in *. 
+      { unfold lookupAs in *. 
         consider (nth_error uenv v); try congruence; intros.
-        erewrite nth_error_weaken in H by eauto.
+        erewrite nth_error_weaken in H0 by eauto.
         consider (typ_eq_odec (projT1 s) t); intros; try congruence.
         subst. inversion H1; inversion H2; clear H1 H2; subst. reflexivity. }
-      { eexists; split; eauto.
-        destruct (IHe1 _ _ _ _ H _ H0 h h0).
-        destruct (IHe2 _ _ _ _ H3 _ H1 h h0).
-        destruct H2; destruct H4.
-        inversion H2; inversion H4; clear H2 H4; subst.
+      { eapply typeof_weaken with (ve := ve) (ue := ue) in H0.
+        rewrite H1 in *.
+        inversion H0; clear H0; subst.
+        specialize (IHe _ _ _ _ H4 H2); clear H2 H4.
+        clear - IHe H5 H3 H.
+        revert H5 H3 IHe. generalize dependent t2. generalize dependent t.
+        induction H; simpl; intros.
+        { destruct (typ_eq_odec t2 t); intros; subst; try congruence.
+          inversion H5; inversion H3; clear H5 H3; subst.
+          eauto. }
+        { destruct t2; try congruence.
+          consider (exprD' fs uenv venv x t2_1); intros; try congruence.
+          consider (exprD' fs (uenv ++ ue) (venv ++ ve) x t2_1); intros; try congruence.
+          specialize (H _ _ _ _ H1 H2 h he); clear H1 H2.
+          specialize (IHForall _ _ _ _ _ _ H5 H3); clear H5 H3 H0.
+          eapply IHForall; intros; simpl in *; clear IHForall.
+          etransitivity. eapply IHe; clear IHe.
+          instantiate (1 := he0). clear - H. admit. } }
+      { simpl; intro. specialize (@IHe _ _ _ _ H H0 (Hcons a h) he); auto. }
+      { specialize (IHe1 _ _ _ _ H H0 h he).
+        specialize (IHe2 _ _ _ _ H3 H1 h he).
         simpl. intuition.
         { etransitivity. symmetry; eauto. etransitivity; eauto. }
         { etransitivity. eauto. etransitivity; eauto. symmetry; eauto. } }
-      { eexists; split; eauto.
-        destruct (IHe _ _ _ _ H _ H0 h h0).
-        destruct H1. inversion H1; clear H1; subst. simpl.
-        intuition; eapply H1; eapply H2; auto. } }
+      { specialize (IHe _ _ _ _ H H0 h he).
+        simpl in *. intuition. }
+  Qed.
+    
+  Theorem exprD_weaken : forall venv e t ue ve x, 
+    exprD fs uenv venv e t = Some x ->
+    exists y, exprD fs (uenv ++ ue) (venv ++ ve) e t = Some y /\
+      equiv ts t x y.
+  Proof.
+    unfold exprD; intros. rewrite split_env_app.
+    destruct (split_env venv). destruct (split_env ve).
+    consider (exprD' fs uenv x0 e t); 
+    consider (exprD' fs (uenv ++ ue) (x0 ++ x1) e t); intros; try congruence.
+    { inversion H1; clear H1; subst.
+      generalize (exprD'_weaken_Some _ _ _ _ _ _ _ H0 H h h0); intros.
+      eexists; split; eauto. }
     { exfalso. inversion H1; clear H1; subst.
       clear - H0 H. generalize dependent t.
       revert x0; revert x1. induction e; simpl; intros;
@@ -200,9 +243,13 @@ Section semantic.
         pattern (nth_error (x0 ++ x1) v) at 2 3.
         erewrite nth_error_weaken by eassumption; intros.
         destruct (typ_eq_odec t1 t); try congruence. }
+      { unfold lookupAs in *.
+        consider (nth_error uenv v); try congruence; intros.
+        erewrite nth_error_weaken in H by eassumption.
+        consider (typ_eq_odec (projT1 s) t); congruence. }
       { erewrite typeof_weaken in H0 by eauto.
         inversion H0; clear H0; subst.
-        generalize (exprD_weaken_Some _ _ _ _ _ _ _ H2 H4).
+        generalize (exprD'_weaken_Some _ _ _ _ _ _ _ H2 H4).
         clear - H5 H3 H.
         generalize dependent t3.
         induction H; simpl; intros.
@@ -211,7 +258,7 @@ Section semantic.
           consider (exprD' fs uenv x0 x t3_1); intros; try congruence.
           consider (exprD' fs (uenv ++ ue) (x0 ++ x1) x t3_1); intros; try congruence.
           { specialize (@IHForall _ _ H5 _ H3). clear H3 H5.
-            generalize (exprD_weaken_Some _ _ _ _ _ _ _ H2 H4); intros.
+            generalize (exprD'_weaken_Some _ _ _ _ _ _ _ H2 H4); intros.
             clear - H1 H3 IHForall. simpl in *.
             eapply IHForall; intros; clear IHForall.
             specialize (H3 h he). specialize (H1 h he).
@@ -223,11 +270,7 @@ Section semantic.
         eapply IHe. eassumption. eapply H2. }
       { eapply typeof_weaken with (ue := ue) (ve := x1) in H1. rewrite H0 in H1.
         congruence. }
-      { eapply IHe; eauto. simpl; eauto. }
-      { unfold lookupAs in *.
-        consider (nth_error uenv v); try congruence; intros.
-        erewrite nth_error_weaken in H by eassumption.
-        consider (typ_eq_odec (projT1 s) t); congruence. } }
+      { eapply IHe; eauto. simpl; eauto. } }
   Qed.
 
 End semantic.
